update

Chapter2/hoare1.lean
@@ -11,18 +11,18 @@ def assertion1 (x y : String): Assertion := fun st => st x ≤ st y
 def assertion2 (x y : String): Assertion := fun st => st x = 3 ∨ st x ≤ st y
 
 def assert_implies (p q : Assertion): Prop := ∀ st, p st → q st
-def assert_iff (p q : Assertion): Prop := ∀ st, p st → q st ∧ q st → p st
+def assert_iff (p q : Assertion): Prop := ∀ st, (p st → q st) ∧ (q st → p st)
 
-def valid_hoare_triple (p q : Assertion) (c : Imp.Command): Prop :=
+def valid_hoare_triple (p : Assertion) (c : Imp.Command) (q: Assertion): Prop :=
   ∀ (st₁ st₂ : Imp.State), Imp.CEval st₁ c st₂ → p st₁ → q st₂
 
 notation p " ->> " q  => assert_implies p q
 notation p " <<->> " q => assert_iff p q
-notation "{" p "} " c " {" q "}" => valid_hoare_triple p q c
+notation "{" p "} " c " {" q "}" => valid_hoare_triple p c q
 
 -- If q holds in every state, then any triple with q as its precondition is valid.
 theorem hoare_post_true : ∀ (p q : Assertion) (c : Imp.Command),
-  (∀ (st : Imp.State), q st) → valid_hoare_triple p q c := by
+  (∀ (st : Imp.State), q st) → valid_hoare_triple p c q := by
   intros p q c hq_st
   unfold valid_hoare_triple
   intros st₁ st₂ hc hp
@@ -30,11 +30,85 @@ theorem hoare_post_true : ∀ (p q : Assertion) (c : Imp.Command),
 
 -- if p holds in no state, then any triple with p as its precondition is valid
 theorem hoare_pre_false : ∀ (p q : Assertion) (c : Imp.Command),
-  (∀ (st : Imp.State), ¬(p st)) → valid_hoare_triple p q c := by
+  (∀ (st : Imp.State), ¬(p st)) → valid_hoare_triple p c q := by
   intros p q c hq_st
   unfold valid_hoare_triple
   intros st₁ st₂ hc hp
   apply hq_st st₁ at hp
   contradiction
+
+theorem hoare_skip : ∀ (p : Assertion), valid_hoare_triple p Imp.Command.skip p := by
+  intro p
+  unfold valid_hoare_triple
+  intros st₁ st₂ hc hp
+  cases hc
+  case skip =>
+    exact hp
+
+theorem hoare_seq : ∀ (p q r : Assertion), ∀ (c₁ c₂ : Imp.Command),
+  valid_hoare_triple q c₂ r → valid_hoare_triple p c₁ q → valid_hoare_triple p (Imp.Command.seq c₁ c₂) r := by
+  intros p q r c₁ c₂ hc₂ hc₁
+  unfold valid_hoare_triple
+  unfold valid_hoare_triple at hc₁
+  unfold valid_hoare_triple at hc₂
+  intros st₁ st₂ hc hp
+  cases hc
+  case seq st₃ hs₁ hs₂ =>
+    apply hc₁ at hs₁
+    apply hc₂ at hs₂
+    apply hs₁ at hp
+    apply hs₂ at hp
+    exact hp
+
+def assertion_sub (p : Assertion) (x : String) (a : Imp.AExp) : Assertion :=
+  fun st => ∀ n, Imp.AEval st a n → p (Imp.set st x n)
+
+notation p " [" x " → " a "]" => assertion_sub p x a
+
+example (x : String):
+  assertion_sub (fun st => st x ≤ 5) x (Imp.AExp.const 3) <<->> (fun st => 3 ≤ 5) := by
+  unfold assert_iff
+  intros st
+  constructor
+  . intro ha
+    simp_all
+  . intro ha
+    unfold assertion_sub
+    intros n he
+    cases he
+    case right.const =>
+      unfold Imp.set
+      simp_all
+
+example (x : String):
+  assertion_sub (fun st => st x ≤ 5) x (.add (.var x) (.const 1)) <<->> (fun st => (st x ) + 1 ≤ 5) := by
+  unfold assert_iff
+  unfold assertion_sub
+  intro st
+  constructor
+  . intro ha
+    specialize ha (st x + 1)
+    unfold Imp.set at ha
+    simp_all
+    apply ha
+    apply Imp.AEval.add
+    apply Imp.AEval.var
+    apply Imp.AEval.const
+  . intro ha n hb
+    unfold Imp.set
+    simp_all
+    cases hb
+    case right.add n₁ n₂ ha₁ ha₂ =>
+      cases ha₂
+      case const =>
+        simp_all
+        cases ha₁
+        case var =>
+          unfold Imp.get
+          exact ha
+
+
+
+
 
 end Hoare1
